work on RWLock

examples/scache/AtomicRefcount.i.dfy
@@ -6,32 +6,31 @@ include "../../lib/Lang/LinearMaybe.s.dfy"
 
 module AtomicRefcountImpl {
   import opened NativeTypes
-  import opened Ptrs
   import opened AtomicSpec
-  import ReadWriteLockResources
+  import RWLock
 
-  type AtomicRefcount = Atomic<uint8, ReadWriteLockResources.Q>
+  type AtomicRefcount = Atomic<uint8, RWLock.R>
 
-  predicate state_inv(v: uint8, g: ReadWriteLockResources.Q, ptr: Ptr, t: int)
+  predicate state_inv(v: uint8, g: RWLock.R, key: RWLock.Key, t: int)
   {
-    g == ReadWriteLockResources.ReadRefCount(ptr, t, v)
+    g == RWLock.Internal(RWLock.ReadRefCount(key, t, v))
   }
 
-  predicate atomic_refcount_inv(a: AtomicRefcount, ptr: Ptr, t: int)
+  predicate atomic_refcount_inv(a: AtomicRefcount, key: RWLock.Key, t: int)
   {
-    forall v, g :: atomic_inv(a, v, g) <==> state_inv(v, g, ptr, t)
+    forall v, g :: atomic_inv(a, v, g) <==> state_inv(v, g, key, t)
   }
 
   method unsafe_obtain<R>() returns (linear r: R)
   method unsafe_dispose<R>(linear r: R)
 
-  method is_refcount_zero(a: AtomicRefcount, ptr: Ptrs.Ptr, t: int,
-      linear m: ReadWriteLockResources.Q)
-  returns (is_zero: bool, linear m': ReadWriteLockResources.Q)
-  requires atomic_refcount_inv(a, ptr, t)
-  requires m == ReadWriteLockResources.WritePending(ptr, t)
-  ensures is_zero ==> m' == ReadWriteLockResources.WritePending(ptr, t + 1)
-  ensures !is_zero ==> m' == ReadWriteLockResources.WritePending(ptr, t)
+  method is_refcount_zero(a: AtomicRefcount, key: RWLock.Key, t: int,
+      linear m: RWLock.R)
+  returns (is_zero: bool, linear m': RWLock.R)
+  requires atomic_refcount_inv(a, key, t)
+  requires m == RWLock.Internal(RWLock.WritePending(key, t))
+  ensures is_zero ==> m' == RWLock.Internal(RWLock.WritePending(key, t + 1))
+  ensures !is_zero ==> m' == RWLock.Internal(RWLock.WritePending(key, t))
   {
     var c := atomic_read(a);
 
@@ -39,15 +38,15 @@ module AtomicRefcountImpl {
     ///// Setup:
     var old_v: uint8;
     var new_v: uint8;
-    linear var old_g: ReadWriteLockResources.Q := unsafe_obtain();
+    linear var old_g: RWLock.R := unsafe_obtain();
     assume new_v == old_v;
     assume c == old_v;
     assume atomic_inv(a, old_v, old_g);
     linear var new_g;
     ///// Transfer:
     if c == 0 {
-      new_g, m' := ReadWriteLockResources.transform_TakeWriteCheckReadZero(
-          ptr, t, old_g, m);
+      new_g, m' := RWLock.transform_TakeWriteCheckReadZero(
+          key, t, old_g, m);
     } else {
       m' := m;
       new_g := old_g;
